Spacetalk/Step.lean
@@ -35,12 +35,13 @@ inductive UnaryOp : Ty → Ty → Type
   | mulConst : {w : Nat} → BitVec w → UnaryOp (BitVecTy w) (BitVecTy w)
 
 inductive Prog : List Ty → Ty → Type
-  | const : (α : Ty) → Prog [α] α
+  | const : {α : Ty} → Prog [α] α
   | zip : BinaryOp α β γ → Prog aInp α → Prog bInp β → Prog (aInp ++ bInp) γ
   | map : UnaryOp α β → Prog inp α → Prog inp β
   | reduce : BinaryOp α β α → Nat → α.denote → Prog inp β → Prog inp α
 
 ------------------ Semantics ------------------
+
 def BinaryOp.denote : BinaryOp α β γ → α.denote → β.denote → γ.denote
   | BinaryOp.add => BitVec.add
   | BinaryOp.mul => BitVec.mul
@@ -50,9 +51,38 @@ def UnaryOp.denote : UnaryOp α β → α.denote → β.denote
   | UnaryOp.mulConst c => BitVec.mul c
 
 def Prog.denote {inputs : List Ty} {α : Ty} : Prog inputs α → (DenoStreamsList inputs → DenoStreamsList [α])
-  | .const α => λ ([a]ₕ) ↦ [a]ₕ
+  | .const => λ ([a]ₕ) ↦ [a]ₕ
   | .zip op as bs => λ inp ↦ let (aInp, bInp) := inp.split; [Stream'.zip op.denote (as.denote aInp).head (bs.denote bInp).head]ₕ
   | .map op as => λ inp ↦ [Stream'.map op.denote (as.denote inp).head]ₕ
   | .reduce op n init bs => λ inp ↦ [Stream'.reduce op.denote n init (bs.denote inp).head]ₕ
+
+------------------ Parser ------------------
+
+declare_syntax_cat step
+
+syntax "const_32" : step
+syntax "const_64" : step
+
+syntax:50 step:50 " +z " step:51 : step
+syntax:60 step:60 " *z " step:61 : step
+
+syntax:40 term "+r" " start " term " on (" step ") " : step
+syntax:40 term "*r" " start " term " on (" step ") " : step
+
+syntax " ( "step " ) " : step
+
+syntax " 〚 " step " 〛 " : term
+
+macro_rules
+  | `(〚 const_32 〛) => `(@Prog.const (BitVecTy 32))
+  | `(〚 const_64 〛) => `(@Prog.const (BitVecTy 64))
+  | `(〚 $a:step +z $b:step 〛) => `(Prog.zip .add 〚 $a 〛 〚 $b 〛)
+  | `(〚 $a:step *z $b:step 〛) => `(Prog.zip .mul 〚 $a 〛 〚 $b 〛)
+  | `(〚 $n:term +r start $init:term on ($a:step) 〛) => `(Prog.reduce .add $n $init 〚 $a 〛)
+  | `(〚 $n:term *r start $init:term on ($a:step) 〛) => `(Prog.reduce .mul $n $init 〚 $a 〛)
+  | `(〚 ( $x ) 〛) => `(〚 $x 〛)
+  | `(〚 $x 〛) => `(〚 $x 〛)
+
+#check 〚 const_32 +z (10 +r start 0 on ((const_32 +z const_32) *z const_32)) 〛
 
 end Step
