Spacetalk/DotProduct.lean
@@ -20,7 +20,7 @@ def sa : Stream' (BitVec 32) := λ n => ⟨n % (2 ^ 32), Nat.mod_lt n (Nat.zero_
 
 namespace Step
   def dotProd (n : Nat) : Prog [BV32, BV32] BV32 :=
-    .reduce .add n 0 (.zip .mul (.const _) (.const _))
+    〚 n +r start 0 on (const_32 *z const_32) 〛
 end Step
 
 theorem step_dp_equiv : ∀n : Nat, (Step.dotProd n).denote = dotProd n := by
