Spacetalk/HList.lean
@@ -20,59 +20,10 @@ inductive Member {α : Type u} : α → List α → Type u
   | tail : Member a bs → Member a (b::bs)
 
 @[simp]
-def Member.toIndex : Member a as → Nat
-  | head => 0
-  | tail m => 1 + m.toIndex
-
-@[simp]
-def Member.compare (m1 : Member a as) (m2 : Member b bs) : Bool :=
-  m1.toIndex == m2.toIndex
-
-@[simp]
-def Member.beq : Member a as → Member a as → Bool
+def Member.compare : Member a as → Member b bs → Bool
   | .head, .head => true
-  | .tail x, .tail y => Member.beq x y
+  | .tail a, .tail b => a.compare b
   | _, _ => false
-
-@[simp]
-instance : BEq (Member a as) where
-  beq := Member.beq
-
-@[simp]
-def Member.decEq : (x : Member a as) → (y : Member a as) → Decidable (x = y)
-  | .head, .head => isTrue rfl
-  | .tail x, .tail y =>
-    match Member.decEq x y with
-    | .isTrue p => isTrue ((Member.tail.injEq x y).to_iff.mpr p)
-    | .isFalse p => isFalse (fun h => p (Member.tail.inj h))
-  | .head, .tail _ => isFalse (fun h => Member.noConfusion h)
-  | .tail _, .head => isFalse (fun h => Member.noConfusion h)
-
-instance : DecidableEq (Member a as) :=
-  Member.decEq
-
-instance : LawfulBEq (Member a as) where
-  rfl := by
-    intro x
-    simp [BEq.beq]
-    induction x with
-    | head => rfl
-    | tail x' ih =>
-      simp [Member.beq]
-      exact ih
-
-  eq_of_beq := by
-    intro x y h
-    induction x
-    cases y
-    · simp
-    · simp [BEq.beq, Member.beq] at h
-    · cases y
-      simp [BEq.beq, Member.beq] at h
-      rename_i a_ih _
-      simp
-      apply a_ih
-      exact h
 
 theorem Member.to_mem : Member a l → a ∈ l
   | .head => List.mem_of_mem_head? rfl
